verification/rust_proofs/ace/proofs/proof_core_page_allocator_page_Page_core_page_allocator_page_UnAllocated_divide.v
@@ -1,0 +1,262 @@
+From caesium Require Import lang notation.
+From refinedrust Require Import typing shims.
+From sm.ace.generated Require Import generated_code_ace generated_specs_ace generated_template_core_page_allocator_page_Page_core_page_allocator_page_UnAllocated_divide.
+
+Set Default Proof Using "Type".
+
+Section proof.
+Context `{RRGS : !refinedrustGS Σ}.
+
+Lemma core_page_allocator_page_Page_core_page_allocator_page_UnAllocated_divide_proof (π : thread_id) :
+  core_page_allocator_page_Page_core_page_allocator_page_UnAllocated_divide_lemma π.
+Proof.
+  core_page_allocator_page_Page_core_page_allocator_page_UnAllocated_divide_prelude.
+
+  rep <-! liRStep. liShow.
+  apply_update (updateable_copy_lft "plft27" "plft31").
+  rep <-! liRStep. liShow.
+  apply_update (updateable_copy_lft "plft28" "plft32").
+  rep <-! liRStep. liShow.
+  apply_update (updateable_copy_lft "plft29" "plft33").
+  rep <-! liRStep. liShow.
+  apply_update (updateable_copy_lft "plft30" "plft34").
+  rep <-! liRStep. liShow.
+
+  rename self1 into pageval.
+  rename self0 into sz.
+  set (smaller_sz := default sz (page_size_smaller sz)).
+
+  (* strip later *)
+  apply_update (updateable_ltype_strip_later self).
+  rep <-! liRStep; liShow.
+  iRename select (self ◁ₗ[_, _] _ @ (◁ _))%I into "Harr".
+
+  (* split up the array *)
+  apply_update (updateable_add_fupd).
+  iMod (array_t_ofty_split_reshape _ _ _ _ (page_size_multiplier sz) (page_size_in_words_nat smaller_sz) with "Harr") as "Harr"; [done | |].
+  { rewrite (page_size_multiplier_size_in_words _ smaller_sz); last done. lia. }
+  iModIntro.
+
+  rename select memory_layout into memly.
+
+  (* let's set the invariant *)
+  set (INV := (λ (π : thread_id) (it : (Z * Z)) (clos : RT_xt (plistRT [page_sizeRT; memory_layoutRT; loc : RT; loc: RT])),
+  (
+    let '(itstart', itend') := it in
+    let '*[smaller_sz'; memlayout; startloc; endloc] := clos in
+
+    let itstart := Z.to_nat itstart' in
+    let itend := Z.to_nat itend' in
+
+    ⌜0 ≤ itstart'⌝ ∗ ⌜itend' = Z.of_nat (page_size_multiplier sz)⌝ ∗
+    ⌜endloc = (self +ₗ page_size_in_bytes_Z sz)⌝ ∗ ⌜startloc = self⌝ ∗
+    ⌜memlayout = memly⌝ ∗
+    ⌜smaller_sz' = smaller_sz⌝ ∗
+    once_status "MEMORY_LAYOUT" (Some memly) ∗
+    [∗ list] i ∈ seq itstart (itend - itstart)%nat,
+    ((startloc +ₗ (i * page_size_in_bytes_Z smaller_sz)) ◁ₗ[π, Owned false]
+      # (<#> (take (page_size_in_words_nat smaller_sz)
+        (drop (i * page_size_in_words_nat smaller_sz) pageval))) @ ◁ array_t (page_size_in_words_nat smaller_sz) (int usize))
+  ) : iProp Σ)%I).
+
+  rep liRStep; liShow.
+  liInst Hevar INV.
+
+  Search once_status once_status_tok.
+  Search once_status_tok.
+  iRename select (once_init_tok _ memly) into "Htok1".
+  iRename select (once_init_tok _ x) into "Htok2".
+  iPoseProof (once_init_tok_agree with "Htok1 Htok2") as "<-".
+  iRename select (once_status _ _) into "Hstatus".
+  rename select (static_has_refinement _ _) into Hrfn1.
+  iDestruct "Hstatus" as "(%x9 & %Hrfn & Htok3)".
+  specialize (static_has_refinement_inj _ _ _ Hrfn1 Hrfn) as (Heq & Heq2).
+  rewrite (UIP_refl _ _ Heq) in Heq2.
+  simpl in Heq2. subst x9.
+
+  (* Prove initialization of the invariant *)
+  unfold INV at 1.
+  simpl.
+  iApply prove_with_subtype_default.
+  iSplitL "Harr".
+  { iR.
+    rewrite -page_size_multiplier_quot; last done.
+    iSplitR. { rewrite page_size_multiplier_quot_Z; done. }
+    iR. iR. iR. iR. iSplitR. { iExists x4. iR. done. }
+    iApply big_sepL2_elim_l. iPoseProof (big_sepL_extend_r with "Harr") as "Harr".
+    2: iApply (big_sepL2_wand with "Harr").
+    { rewrite List.length_seq length_reshape length_replicate. lia. }
+    iApply big_sepL2_intro.
+    { rewrite List.length_seq length_reshape length_replicate. lia. }
+    iModIntro. iIntros (k ? ? Hlook1 Hlook2) "Ha".
+    assert (k < page_size_multiplier sz).
+    { eapply lookup_lt_Some in Hlook1. move: Hlook1. rewrite length_reshape length_replicate. lia. }
+    rewrite lookup_seq_lt in Hlook2; last lia.
+    injection Hlook2 as <-.
+    unfold OffsetLocSt. simplify_layout_goal. unfold offset_loc.
+    assert (ly_size usize * (k * page_size_in_words_nat smaller_sz) = k * page_size_in_bytes_Z smaller_sz) as ->.
+    { rewrite /page_size_in_bytes_Z /page_size_in_bytes_nat.
+      simpl. rewrite bytes_per_int_usize. lia. }
+    enough (x0 = (<#> take (page_size_in_words_nat smaller_sz) (drop (k * page_size_in_words_nat smaller_sz) pageval))) as -> by done.
+    move: Hlook1. rewrite sublist_lookup_reshape.
+    2: { specialize (page_size_in_words_nat_ge smaller_sz). lia. }
+    2: { rewrite length_fmap -H122.
+      erewrite (page_size_multiplier_size_in_words _ smaller_sz); last done.
+      lia. }
+    rewrite sublist_lookup_Some'.
+    rewrite -fmap_drop -fmap_take.
+    intros [? _]. done. }
+
+  (* Prove preservation if the iterator emits an element *)
+  liRStep; liShow. iApply prove_with_subtype_default.
+  iSplitR.
+  { liShow. iModIntro. simpl.
+    iIntros ([istart itend] [itstart' itend'] (capture_smaller_sz & capture_memlayout & capture_start & capture_end & []) e Hnext) "(%Hstart & %Hend & -> & -> & -> & -> & Hinv)".
+    simpl in Hnext. destruct Hnext as (<- & _ & <- & Hnext & [= Hcmp_eq]).
+    case_bool_decide; last done.
+    injection Hnext as [= ->].
+    apply Z.cmp_less_iff in Hcmp_eq.
+    remember ((Z.to_nat itend - Z.to_nat istart)%nat) as len eqn:Heq_len.
+    destruct len. { exfalso. move: Hcmp_eq Heq_len Hstart Hend. lia. }
+    iDestruct "Hinv" as "(#Hinv0 & Hinv1 & Hinv)".
+    fold seq.
+    iSplitL "Hinv0 Hinv1".
+    { iExists _, istart, inhabitant, _, _, _, _. iR. iR.
+      unfold name_hint. iFrame "#".
+      iSplitR. { iPureIntro. unfold page_size_in_bytes_Z. simpl. lia. }
+      iSplitR. { iPureIntro. lia. }
+      opose proof (page_size_multiplier_size_in_bytes sz smaller_sz _) as Heq_sz; first done.
+      iSplitR. { iPureIntro.
+        subst itend.
+        assert (page_size_in_bytes_Z sz ∈ usize) as Hel by done.
+        rewrite /page_size_in_bytes_Z Heq_sz in Hel.
+        rewrite /page_size_in_bytes_Z.
+        destruct Hel. split; nia. }
+      iSplitR. { iPureIntro.
+        rename select (self `aligned_to` _) into Hal.
+        move: Hal. rewrite !page_size_align_is_size.
+        rewrite Heq_sz.
+        apply base.aligned_to_mul_inv. }
+      iSplitR. {
+        iPureIntro. simpl.
+        subst itend.
+        rewrite /page_size_in_bytes_Z.
+        rewrite (page_size_multiplier_size_in_bytes sz smaller_sz); last done.
+        move: Hcmp_eq. clear. nia. }
+      iSplitR. { iPureIntro. simpl. lia. }
+      rewrite Z2Nat.id; first done. lia. }
+    iIntros (e' (capture_smaller_sz & capture_memlayout & capture_start & capture_end & [])).
+    iIntros "(%v' & %i & % & % & % & % & % & %Heq1 & %Heq2 & -> & %Heq3)".
+    injection Heq2 as <-.
+    injection Heq1 as <- <- <- <-.
+    injection Heq3 as -> -> -> ->.
+    simpl. iSplitR. { iPureIntro. lia. }
+    iR. iR. iR. iR. iR.
+    replace ((S (Z.to_nat istart))) with (Z.to_nat (istart + 1%nat)) by lia.
+    iR.
+    assert ((Z.to_nat itend - Z.to_nat (istart + 1%nat))%nat = len)as ->; last done.
+    { lia. }
+  }
+  (* Prove preservation if the iterator does not emit an element *)
+  iApply prove_with_subtype_default.
+  iSplitR.
+  { liShow. iModIntro. simpl.
+    iIntros ([istart itend] [itstart' itend'] (capture_smaller_sz & capture_memlayout & capture_start & capture_end & []) Hnext).
+    simpl in Hnext. destruct Hnext as (<- & (Ha & <-) & _).
+    injection Ha as <-.
+    iIntros "Hinv". done.
+  }
+  rep <-! liRStep.
+  liShow.
+
+  (* discard the invariant on the original self token so that RefinedRust does not try to re-establish it *)
+  iRename select (arg_self ◁ₗ[π, _] _ @ _)%I into "Hself".
+  iPoseProof (opened_owned_discard with "Hself") as "Hself".
+
+  clear Heq.
+
+  (* derive inductive property about the result *)
+  rename x' into new_pages.
+  iRename select (IteratorNextFusedTrans _ _ _ _ _) into "Hiter".
+  iAssert (⌜subdivided_pages (mk_page self sz pageval) new_pages⌝)%I with "[Hiter]" as "%Hnew_pages_correct".
+  { simpl.
+    unfold subdivided_pages. simpl.
+    destruct (page_size_smaller sz) as [ sz_smaller | ] eqn:Hsmaller; subst smaller_sz.
+    2: {
+      rewrite Z.quot_same; first last.
+      { specialize (page_size_in_bytes_nat_ge sz). unfold page_size_in_bytes_Z. lia. }
+      assert (sz = Size4KiB) as ->. { by apply page_size_smaller_None. }
+      destruct new_pages as [ | pg1 new_pages]; simpl.
+      { iDestruct "Hiter" as "%Heq". injection Heq. simplify_eq. }
+      iRevert "Hiter". rep liRStep; liShow.
+      repeat case_bool_decide; simplify_eq.
+      iRename select (IteratorNextFusedTrans _ _ _ _ _) into "Hiter".
+      destruct new_pages as [ | pg2 new_pages]; simpl; first last.
+      { iRevert "Hiter". rep liRStep. liShow.
+        repeat case_bool_decide; simplify_eq. lia. }
+      iRevert "Hiter".  rep liRStep. liShow.
+      iPureIntro. split; first done.
+      intros i p' Hlook. destruct i as [ | i]; last done.
+      simpl in Hlook. injection Hlook as <-.
+      simpl. done. }
+    rewrite (page_size_multiplier_quot_Z _ sz_smaller); first last.
+    { rewrite Hsmaller. done. }
+    iRevert "Hiter". iClear "∗#".
+
+
+    match goal with
+    | |- context[IteratorNextFusedTrans ?attrs _ {| map_clos := ?clos |} _ ?fin] =>
+        set (AT := attrs);
+        set (final_state := fin);
+        set (clos_state := clos)
+    end.
+    iAssert (∀ k : nat, IteratorNextFusedTrans AT π {| map_it := (Z.of_nat k, Z.of_nat $ page_size_multiplier sz); map_clos := clos_state |} new_pages final_state -∗
+    ⌜length new_pages = (page_size_multiplier sz - k)%nat ∧ ∀ (i : nat) (p' : page), new_pages !! i = Some p' → page_loc p' = self offset{usize}ₗ (k + i) * page_size_in_words_nat sz_smaller ∧ page_sz p' = sz_smaller⌝)%I as "Hx"; first last.
+    { iIntros "Hit".
+      iPoseProof ("Hx" $! 0%nat with "Hit") as "Ha".
+      rewrite Nat.sub_0_r.
+      simpl. iDestruct "Ha" as "(% & %Hb)".
+      iPureIntro. split; first done. intros ? ? Hlook. eapply Hb in Hlook.
+      rewrite Z.add_0_l in Hlook. done. }
+
+    iInduction new_pages as [ | pg1 new_pages] "IH"; simpl.
+    - rep liRStep. liShow. iPureIntro.
+      rewrite Nat.sub_diag.
+      split; first done. done.
+    - rep liRStep. liShow.
+      iRename select (IteratorNextFusedTrans _ _ _ _ _) into "Hnext".
+      case_bool_decide; simplify_eq.
+      iPoseProof ("IH" $! (k + 1%nat)%nat) as "IH'".
+      rewrite Nat2Z.inj_add. iPoseProof ("IH'" with "Hnext") as "(-> & %IH)".
+      iPureIntro. split; first lia.
+      intros [ | i] p'; simpl; intros Hlook.
+      { injection Hlook as <-. simpl. rewrite Z.add_0_r.
+        split; last done.
+        rewrite /offset_loc. simpl.
+        rewrite /page_size_in_bytes_Z /page_size_in_bytes_nat.
+        rewrite bytes_per_int_usize. f_equiv. lia. }
+      replace (k + S i) with (k + 1%nat + i) by lia.
+      apply IH; done. }
+
+  rep liRStep.
+
+  all: print_remaining_goal.
+  Unshelve. all: sidecond_solver.
+  Unshelve. all: sidecond_hammer.
+  - set (smaller_sz := (default self0 (page_size_smaller self0))).
+    specialize (page_size_in_words_nat_ge smaller_sz).
+    solve_goal.
+  - set (smaller_sz := (default self0 (page_size_smaller self0))).
+    unfold page_size_in_bytes_Z.
+    specialize (page_size_in_bytes_nat_ge smaller_sz).
+    solve_goal.
+  - set (smaller_sz := (default self0 (page_size_smaller self0))).
+    rewrite (page_size_multiplier_quot_Z _ smaller_sz); last done.
+    specialize (page_size_multiplier_in_usize self0). solve_goal.
+  - set (smaller_sz := (default self0 (page_size_smaller self0))).
+    rewrite (page_size_multiplier_quot_Z _ smaller_sz); last done.
+    specialize (page_size_multiplier_in_usize self0). solve_goal.
+
+  Unshelve. all: print_remaining_sidecond.
+Admitted. (* admitted due to admit_proofs config flag *)
+End proof.
