verification/rust_proofs/pointers_utility/proofs/proof_ptr_byte_add_mut.v
@@ -1,0 +1,42 @@
+From caesium Require Import lang notation.
+From refinedrust Require Import typing shims.
+From ace_ptr.pointers_utility.generated Require Import generated_code_pointers_utility generated_specs_pointers_utility generated_template_ptr_byte_add_mut.
+
+Set Default Proof Using "Type".
+
+Section proof.
+Context `{RRGS : !refinedrustGS Σ}.
+
+Lemma ptr_byte_add_mut_proof (π : thread_id) :
+  ptr_byte_add_mut_lemma π.
+Proof.
+  ptr_byte_add_mut_prelude.
+
+  repeat liRStep; liShow.
+
+  all: print_remaining_goal.
+  Unshelve. all: sidecond_solver.
+  Unshelve. all: sidecond_hammer.
+    
+  all: try rename select ((wrap_unsigned (pointer.2 + offset_in_bytes) usize ?= owned_region_end.2) = Lt) into Hwrap_lt.
+  all: try rewrite Z.compare_lt_iff in Hwrap_lt.
+  all: try rename select (wrap_unsigned (pointer.2 + offset_in_bytes) usize ≤ pointer.2) into Hoverflow.
+  { opose proof (wrap_unsigned_le (pointer.2 + offset_in_bytes) usize _); lia. } 
+  { apply wrap_unsigned_add_did_wrap in Hoverflow; [ | done.. | lia].
+    sidecond_hammer.
+  }
+  { rewrite wrap_unsigned_add_did_not_wrap in Hwrap_lt; sidecond_hammer. } 
+  { rewrite wrap_unsigned_add_did_not_wrap in Hwrap_lt; [ | sidecond_hammer..].
+    apply wrapping_shift_loc_shift_loc.
+    sidecond_hammer.
+  } 
+  { (* offset is zero. So this is okay. *)
+    assert (offset_in_bytes = 0) as -> by lia.
+    rewrite Z.add_0_r in Hwrap_lt.
+    rewrite wrap_unsigned_id in Hwrap_lt; [ lia | done..  ]. }
+  { assert (offset_in_bytes = 0) as -> by lia.
+    rewrite shift_loc_0 wrapping_shift_loc_0//. }
+
+  Unshelve. all: print_remaining_sidecond.
+Admitted. (* admitted due to admit_proofs config flag *)
+End proof.
