verification/theories/memory_layout/memory_layout.v
@@ -7,7 +7,15 @@ Record memory_layout : Type := mk_memory_layout {
   conf_end : loc;
   non_conf_start : loc;
   non_conf_end : loc;
-}.
 
-Global Instance memory_layout_inhabited : Inhabited memory_layout :=
-  populate (mk_memory_layout inhabitant inhabitant inhabitant inhabitant).
+  conf_start_in_usize : conf_start.2 ∈ usize;
+  conf_end_in_usize : conf_end.2 ∈ usize;
+  non_conf_start_in_usize : non_conf_start.2 ∈ usize;
+  non_conf_end_in_usize : non_conf_end.2 ∈ usize;
+}.
+Canonical Structure memory_layoutRT := directRT memory_layout. 
+
+Global Program Instance memory_layout_inhabited : Inhabited memory_layout :=
+  populate (mk_memory_layout 
+    NULL_loc NULL_loc NULL_loc NULL_loc _ _ _ _).
+Solve Obligations with split; unsafe_unfold_common_caesium_defs; sidecond_hammer.
